moving greek suffixes to proper names

Expressiveness_Price.thy
@@ -63,127 +63,127 @@ lemma "modal_depth_srbb (ImmConj \<nat> (\<lambda>n. Pos (Obs \<alpha> (observe_
 subsection \<open>Depth of branching conjunctions\<close>
 
 primrec branching_conjunction_depth :: "('a, 's) hml_srbb \<Rightarrow> enat"
-  and branch_conj_depth_\<chi> :: "('a, 's) hml_srbb_inner \<Rightarrow> enat"
-  and branch_conj_depth_\<psi> :: "('a, 's) hml_srbb_conjunct \<Rightarrow> enat" where
+  and branch_conj_depth_inner :: "('a, 's) hml_srbb_inner \<Rightarrow> enat"
+  and branch_conj_depth_conjunct :: "('a, 's) hml_srbb_conjunct \<Rightarrow> enat" where
   "branching_conjunction_depth TT = 0" |
-  "branching_conjunction_depth (Internal \<chi>) = branch_conj_depth_\<chi> \<chi>" |
-  "branching_conjunction_depth (ImmConj I \<psi>s) = Sup ((branch_conj_depth_\<psi> \<circ> \<psi>s) ` I)" |
+  "branching_conjunction_depth (Internal \<chi>) = branch_conj_depth_inner \<chi>" |
+  "branching_conjunction_depth (ImmConj I \<psi>s) = Sup ((branch_conj_depth_conjunct \<circ> \<psi>s) ` I)" |
 
-  "branch_conj_depth_\<chi> (Obs _ \<phi>) = branching_conjunction_depth \<phi>" |
-  "branch_conj_depth_\<chi> (Conj I \<psi>s) = Sup ((branch_conj_depth_\<psi> \<circ> \<psi>s) ` I)" |
-  "branch_conj_depth_\<chi> (StableConj I \<psi>s) = Sup ((branch_conj_depth_\<psi> \<circ> \<psi>s) ` I)" |
-  "branch_conj_depth_\<chi> (BranchConj _ \<phi> I \<psi>s) = 1 + Sup ({branching_conjunction_depth \<phi>} \<union> ((branch_conj_depth_\<psi> \<circ> \<psi>s) ` I))" |
+  "branch_conj_depth_inner (Obs _ \<phi>) = branching_conjunction_depth \<phi>" |
+  "branch_conj_depth_inner (Conj I \<psi>s) = Sup ((branch_conj_depth_conjunct \<circ> \<psi>s) ` I)" |
+  "branch_conj_depth_inner (StableConj I \<psi>s) = Sup ((branch_conj_depth_conjunct \<circ> \<psi>s) ` I)" |
+  "branch_conj_depth_inner (BranchConj _ \<phi> I \<psi>s) = 1 + Sup ({branching_conjunction_depth \<phi>} \<union> ((branch_conj_depth_conjunct \<circ> \<psi>s) ` I))" |
 
-  "branch_conj_depth_\<psi> (Pos \<chi>) = branch_conj_depth_\<chi> \<chi>" |
-  "branch_conj_depth_\<psi> (Neg \<chi>) = branch_conj_depth_\<chi> \<chi>" 
+  "branch_conj_depth_conjunct (Pos \<chi>) = branch_conj_depth_inner \<chi>" |
+  "branch_conj_depth_conjunct (Neg \<chi>) = branch_conj_depth_inner \<chi>" 
 
 subsection \<open>Depth of instable conjunctions\<close>
 
 primrec
 instable_conjunction_depth :: "('a, 's) hml_srbb \<Rightarrow> enat"
-  and inst_conj_depth_\<chi> :: "('a, 's) hml_srbb_inner \<Rightarrow> enat"
-  and inst_conj_depth_\<psi> :: "('a, 's) hml_srbb_conjunct \<Rightarrow> enat" where
+  and inst_conj_depth_inner :: "('a, 's) hml_srbb_inner \<Rightarrow> enat"
+  and inst_conj_depth_conjunct :: "('a, 's) hml_srbb_conjunct \<Rightarrow> enat" where
   "instable_conjunction_depth TT = 0" |
-  "instable_conjunction_depth (Internal \<chi>) = inst_conj_depth_\<chi> \<chi>" |
-  "instable_conjunction_depth (ImmConj I \<psi>s) = 1 + Sup ((inst_conj_depth_\<psi> \<circ> \<psi>s) ` I)" |
+  "instable_conjunction_depth (Internal \<chi>) = inst_conj_depth_inner \<chi>" |
+  "instable_conjunction_depth (ImmConj I \<psi>s) = 1 + Sup ((inst_conj_depth_conjunct \<circ> \<psi>s) ` I)" |
 
-  "inst_conj_depth_\<chi> (Obs _ \<phi>) = instable_conjunction_depth \<phi>" |
-  "inst_conj_depth_\<chi> (Conj I \<psi>s) = 1 + Sup ((inst_conj_depth_\<psi> \<circ> \<psi>s) ` I)" |
-  "inst_conj_depth_\<chi> (StableConj I \<psi>s) = Sup ((inst_conj_depth_\<psi> \<circ> \<psi>s) ` I)" |
-  "inst_conj_depth_\<chi> (BranchConj _ \<phi> I \<psi>s) = Sup ({instable_conjunction_depth \<phi>} \<union> ((inst_conj_depth_\<psi> \<circ> \<psi>s) ` I))" |
+  "inst_conj_depth_inner (Obs _ \<phi>) = instable_conjunction_depth \<phi>" |
+  "inst_conj_depth_inner (Conj I \<psi>s) = 1 + Sup ((inst_conj_depth_conjunct \<circ> \<psi>s) ` I)" |
+  "inst_conj_depth_inner (StableConj I \<psi>s) = Sup ((inst_conj_depth_conjunct \<circ> \<psi>s) ` I)" |
+  "inst_conj_depth_inner (BranchConj _ \<phi> I \<psi>s) = Sup ({instable_conjunction_depth \<phi>} \<union> ((inst_conj_depth_conjunct \<circ> \<psi>s) ` I))" |
 
-  "inst_conj_depth_\<psi> (Pos \<chi>) = inst_conj_depth_\<chi> \<chi>" |
-  "inst_conj_depth_\<psi> (Neg \<chi>) = inst_conj_depth_\<chi> \<chi>" 
+  "inst_conj_depth_conjunct (Pos \<chi>) = inst_conj_depth_inner \<chi>" |
+  "inst_conj_depth_conjunct (Neg \<chi>) = inst_conj_depth_inner \<chi>" 
 
 subsection \<open>Depth of stable conjunctions\<close>
 
 primrec
 stable_conjunction_depth :: "('a, 's) hml_srbb \<Rightarrow> enat"
-  and st_conj_depth_\<chi> :: "('a, 's) hml_srbb_inner \<Rightarrow> enat"
-  and st_conj_depth_\<psi> :: "('a, 's) hml_srbb_conjunct \<Rightarrow> enat" where
+  and st_conj_depth_inner :: "('a, 's) hml_srbb_inner \<Rightarrow> enat"
+  and st_conj_depth_conjunct :: "('a, 's) hml_srbb_conjunct \<Rightarrow> enat" where
   "stable_conjunction_depth TT = 0" |
-  "stable_conjunction_depth (Internal \<chi>) = st_conj_depth_\<chi> \<chi>" |
-  "stable_conjunction_depth (ImmConj I \<psi>s) = Sup ((st_conj_depth_\<psi> \<circ> \<psi>s) ` I)" |
+  "stable_conjunction_depth (Internal \<chi>) = st_conj_depth_inner \<chi>" |
+  "stable_conjunction_depth (ImmConj I \<psi>s) = Sup ((st_conj_depth_conjunct \<circ> \<psi>s) ` I)" |
 
-  "st_conj_depth_\<chi> (Obs _ \<phi>) = stable_conjunction_depth \<phi>" |
-  "st_conj_depth_\<chi> (Conj I \<psi>s) = Sup ((st_conj_depth_\<psi> \<circ> \<psi>s) ` I)" |
-  "st_conj_depth_\<chi> (StableConj I \<psi>s) = 1 + Sup ((st_conj_depth_\<psi> \<circ> \<psi>s) ` I)" |
-  "st_conj_depth_\<chi> (BranchConj _ \<phi> I \<psi>s) = Sup ({stable_conjunction_depth \<phi>} \<union> ((st_conj_depth_\<psi> \<circ> \<psi>s) ` I))" |
+  "st_conj_depth_inner (Obs _ \<phi>) = stable_conjunction_depth \<phi>" |
+  "st_conj_depth_inner (Conj I \<psi>s) = Sup ((st_conj_depth_conjunct \<circ> \<psi>s) ` I)" |
+  "st_conj_depth_inner (StableConj I \<psi>s) = 1 + Sup ((st_conj_depth_conjunct \<circ> \<psi>s) ` I)" |
+  "st_conj_depth_inner (BranchConj _ \<phi> I \<psi>s) = Sup ({stable_conjunction_depth \<phi>} \<union> ((st_conj_depth_conjunct \<circ> \<psi>s) ` I))" |
 
-  "st_conj_depth_\<psi> (Pos \<chi>) = st_conj_depth_\<chi> \<chi>" |
-  "st_conj_depth_\<psi> (Neg \<chi>) = st_conj_depth_\<chi> \<chi>" 
+  "st_conj_depth_conjunct (Pos \<chi>) = st_conj_depth_inner \<chi>" |
+  "st_conj_depth_conjunct (Neg \<chi>) = st_conj_depth_inner \<chi>" 
 
 subsection \<open>Depth of immediate conjunctions\<close>
 
 primrec
       immediate_conjunction_depth :: "('a, 's) hml_srbb \<Rightarrow> enat"
-  and imm_conj_depth_\<chi> :: "('a, 's) hml_srbb_inner \<Rightarrow> enat"
-  and imm_conj_depth_\<psi> :: "('a, 's) hml_srbb_conjunct \<Rightarrow> enat" where 
+  and imm_conj_depth_inner :: "('a, 's) hml_srbb_inner \<Rightarrow> enat"
+  and imm_conj_depth_conjunct :: "('a, 's) hml_srbb_conjunct \<Rightarrow> enat" where 
   "immediate_conjunction_depth TT = 0" |
-  "immediate_conjunction_depth (Internal \<chi>) = imm_conj_depth_\<chi> \<chi>" |
-  "immediate_conjunction_depth (ImmConj I \<psi>s) = 1 + Sup ((imm_conj_depth_\<psi> \<circ> \<psi>s) ` I)" |
+  "immediate_conjunction_depth (Internal \<chi>) = imm_conj_depth_inner \<chi>" |
+  "immediate_conjunction_depth (ImmConj I \<psi>s) = 1 + Sup ((imm_conj_depth_conjunct \<circ> \<psi>s) ` I)" |
 
-  "imm_conj_depth_\<chi> (Obs _ \<phi>) = immediate_conjunction_depth \<phi>" |
-  "imm_conj_depth_\<chi> (Conj I \<psi>s) = Sup ((imm_conj_depth_\<psi> \<circ> \<psi>s) ` I)" |
-  "imm_conj_depth_\<chi> (StableConj I \<psi>s) = Sup ((imm_conj_depth_\<psi> \<circ> \<psi>s) ` I)" |
-  "imm_conj_depth_\<chi> (BranchConj _ \<phi> I \<psi>s) = Sup ({immediate_conjunction_depth \<phi>} \<union> ((imm_conj_depth_\<psi> \<circ> \<psi>s) ` I))" |
+  "imm_conj_depth_inner (Obs _ \<phi>) = immediate_conjunction_depth \<phi>" |
+  "imm_conj_depth_inner (Conj I \<psi>s) = Sup ((imm_conj_depth_conjunct \<circ> \<psi>s) ` I)" |
+  "imm_conj_depth_inner (StableConj I \<psi>s) = Sup ((imm_conj_depth_conjunct \<circ> \<psi>s) ` I)" |
+  "imm_conj_depth_inner (BranchConj _ \<phi> I \<psi>s) = Sup ({immediate_conjunction_depth \<phi>} \<union> ((imm_conj_depth_conjunct \<circ> \<psi>s) ` I))" |
 
-  "imm_conj_depth_\<psi> (Pos \<chi>) = imm_conj_depth_\<chi> \<chi>" |
-  "imm_conj_depth_\<psi> (Neg \<chi>) = imm_conj_depth_\<chi> \<chi>"
+  "imm_conj_depth_conjunct (Pos \<chi>) = imm_conj_depth_inner \<chi>" |
+  "imm_conj_depth_conjunct (Neg \<chi>) = imm_conj_depth_inner \<chi>"
 
 section \<open>Maximal modal depth of positive clauses in conjunctions\<close>
 
 primrec
       max_positive_conjunct_depth :: "('a, 's) hml_srbb \<Rightarrow> enat"
-  and max_pos_conj_depth_\<chi> :: "('a, 's) hml_srbb_inner \<Rightarrow> enat"
-  and max_pos_conj_depth_\<psi> :: "('a, 's) hml_srbb_conjunct \<Rightarrow> enat" where
+  and max_pos_conj_depth_inner :: "('a, 's) hml_srbb_inner \<Rightarrow> enat"
+  and max_pos_conj_depth_conjunct :: "('a, 's) hml_srbb_conjunct \<Rightarrow> enat" where
   "max_positive_conjunct_depth TT = 0"|
-  "max_positive_conjunct_depth (Internal \<chi>) = max_pos_conj_depth_\<chi> \<chi>" |
-  "max_positive_conjunct_depth (ImmConj I \<psi>s) = Sup ((max_pos_conj_depth_\<psi> \<circ> \<psi>s) ` I)" |
+  "max_positive_conjunct_depth (Internal \<chi>) = max_pos_conj_depth_inner \<chi>" |
+  "max_positive_conjunct_depth (ImmConj I \<psi>s) = Sup ((max_pos_conj_depth_conjunct \<circ> \<psi>s) ` I)" |
 
-  "max_pos_conj_depth_\<chi> (Obs _ \<phi>) = max_positive_conjunct_depth \<phi>" |
-  "max_pos_conj_depth_\<chi> (Conj I \<psi>s) = Sup ((max_pos_conj_depth_\<psi> \<circ> \<psi>s) ` I)" |
-  "max_pos_conj_depth_\<chi> (StableConj I \<psi>s) = Sup ((max_pos_conj_depth_\<psi> \<circ> \<psi>s) ` I)" |
-  "max_pos_conj_depth_\<chi> (BranchConj _ \<phi> I \<psi>s) = Sup ({max_positive_conjunct_depth \<phi>} \<union> ((max_pos_conj_depth_\<psi> \<circ> \<psi>s) ` I))" |
+  "max_pos_conj_depth_inner (Obs _ \<phi>) = max_positive_conjunct_depth \<phi>" |
+  "max_pos_conj_depth_inner (Conj I \<psi>s) = Sup ((max_pos_conj_depth_conjunct \<circ> \<psi>s) ` I)" |
+  "max_pos_conj_depth_inner (StableConj I \<psi>s) = Sup ((max_pos_conj_depth_conjunct \<circ> \<psi>s) ` I)" |
+  "max_pos_conj_depth_inner (BranchConj _ \<phi> I \<psi>s) = Sup ({max_positive_conjunct_depth \<phi>} \<union> ((max_pos_conj_depth_conjunct \<circ> \<psi>s) ` I))" |
 
-  "max_pos_conj_depth_\<psi> (Pos \<chi>) = modal_depth_srbb_inner \<chi>" |
-  "max_pos_conj_depth_\<psi> (Neg \<chi>) = max_pos_conj_depth_\<chi> \<chi>"
+  "max_pos_conj_depth_conjunct (Pos \<chi>) = modal_depth_srbb_inner \<chi>" |
+  "max_pos_conj_depth_conjunct (Neg \<chi>) = max_pos_conj_depth_inner \<chi>"
 
 subsection \<open>Maximal modal depth of negative clauses in conjunctions\<close>
 
 primrec
       max_negative_conjunct_depth :: "('a, 's) hml_srbb \<Rightarrow> enat"
-  and max_neg_conj_depth_\<chi> :: "('a, 's) hml_srbb_inner \<Rightarrow> enat"
-  and max_neg_conj_depth_\<psi> :: "('a, 's) hml_srbb_conjunct \<Rightarrow> enat" where
+  and max_neg_conj_depth_inner :: "('a, 's) hml_srbb_inner \<Rightarrow> enat"
+  and max_neg_conj_depth_conjunct :: "('a, 's) hml_srbb_conjunct \<Rightarrow> enat" where
   "max_negative_conjunct_depth TT = 0" |
-  "max_negative_conjunct_depth (Internal \<chi>) = max_neg_conj_depth_\<chi> \<chi>" |
-  "max_negative_conjunct_depth (ImmConj I \<psi>s) = Sup ((max_neg_conj_depth_\<psi> \<circ> \<psi>s) ` I)" |
+  "max_negative_conjunct_depth (Internal \<chi>) = max_neg_conj_depth_inner \<chi>" |
+  "max_negative_conjunct_depth (ImmConj I \<psi>s) = Sup ((max_neg_conj_depth_conjunct \<circ> \<psi>s) ` I)" |
 
-  "max_neg_conj_depth_\<chi> (Obs _ \<phi>) = max_negative_conjunct_depth \<phi>" |
-  "max_neg_conj_depth_\<chi> (Conj I \<psi>s) = Sup ((max_neg_conj_depth_\<psi> \<circ> \<psi>s) ` I)" |
-  "max_neg_conj_depth_\<chi> (StableConj I \<psi>s) = Sup ((max_neg_conj_depth_\<psi> \<circ> \<psi>s) ` I)" |
-  "max_neg_conj_depth_\<chi> (BranchConj _ \<phi> I \<psi>s) = Sup ({max_negative_conjunct_depth \<phi>} \<union> ((max_neg_conj_depth_\<psi> \<circ> \<psi>s) ` I))" |
+  "max_neg_conj_depth_inner (Obs _ \<phi>) = max_negative_conjunct_depth \<phi>" |
+  "max_neg_conj_depth_inner (Conj I \<psi>s) = Sup ((max_neg_conj_depth_conjunct \<circ> \<psi>s) ` I)" |
+  "max_neg_conj_depth_inner (StableConj I \<psi>s) = Sup ((max_neg_conj_depth_conjunct \<circ> \<psi>s) ` I)" |
+  "max_neg_conj_depth_inner (BranchConj _ \<phi> I \<psi>s) = Sup ({max_negative_conjunct_depth \<phi>} \<union> ((max_neg_conj_depth_conjunct \<circ> \<psi>s) ` I))" |
 
-  "max_neg_conj_depth_\<psi> (Pos \<chi>) = max_neg_conj_depth_\<chi> \<chi>" |
-  "max_neg_conj_depth_\<psi> (Neg \<chi>) = modal_depth_srbb_inner \<chi>"
+  "max_neg_conj_depth_conjunct (Pos \<chi>) = max_neg_conj_depth_inner \<chi>" |
+  "max_neg_conj_depth_conjunct (Neg \<chi>) = modal_depth_srbb_inner \<chi>"
 
 subsection \<open>Depth of negations\<close>
 
 primrec
       negation_depth :: "('a, 's) hml_srbb \<Rightarrow> enat"
-  and neg_depth_\<chi> :: "('a, 's) hml_srbb_inner \<Rightarrow> enat"
-  and neg_depth_\<psi> :: "('a, 's) hml_srbb_conjunct \<Rightarrow> enat" where
+  and neg_depth_inner :: "('a, 's) hml_srbb_inner \<Rightarrow> enat"
+  and neg_depth_conjunct :: "('a, 's) hml_srbb_conjunct \<Rightarrow> enat" where
   "negation_depth TT = 0" |
-  "negation_depth (Internal \<chi>) = neg_depth_\<chi> \<chi>" |
-  "negation_depth (ImmConj I \<psi>s) = Sup ((neg_depth_\<psi> \<circ> \<psi>s) ` I)" |
+  "negation_depth (Internal \<chi>) = neg_depth_inner \<chi>" |
+  "negation_depth (ImmConj I \<psi>s) = Sup ((neg_depth_conjunct \<circ> \<psi>s) ` I)" |
 
-  "neg_depth_\<chi> (Obs _ \<phi>) = negation_depth \<phi>" |
-  "neg_depth_\<chi> (Conj I \<psi>s) = Sup ((neg_depth_\<psi> \<circ> \<psi>s) ` I)" |
-  "neg_depth_\<chi> (StableConj I \<psi>s) = Sup ((neg_depth_\<psi> \<circ> \<psi>s) ` I)" |
-  "neg_depth_\<chi> (BranchConj _ \<phi> I \<psi>s) = Sup ({negation_depth \<phi>} \<union> ((neg_depth_\<psi> \<circ> \<psi>s) ` I))" |
+  "neg_depth_inner (Obs _ \<phi>) = negation_depth \<phi>" |
+  "neg_depth_inner (Conj I \<psi>s) = Sup ((neg_depth_conjunct \<circ> \<psi>s) ` I)" |
+  "neg_depth_inner (StableConj I \<psi>s) = Sup ((neg_depth_conjunct \<circ> \<psi>s) ` I)" |
+  "neg_depth_inner (BranchConj _ \<phi> I \<psi>s) = Sup ({negation_depth \<phi>} \<union> ((neg_depth_conjunct \<circ> \<psi>s) ` I))" |
 
-  "neg_depth_\<psi> (Pos \<chi>) = neg_depth_\<chi> \<chi>" |
-  "neg_depth_\<psi> (Neg \<chi>) = 1 + neg_depth_\<chi> \<chi>" 
+  "neg_depth_conjunct (Pos \<chi>) = neg_depth_inner \<chi>" |
+  "neg_depth_conjunct (Neg \<chi>) = 1 + neg_depth_inner \<chi>" 
 
 subsection \<open>Expressiveness price function\<close>
 
@@ -203,21 +203,21 @@ lemma srbb_price_never_neg : "expressiveness_price \<phi> \<noteq> eneg"
 definition \<O> :: "energy \<Rightarrow> (('a, 's) hml_srbb) set" where
   "\<O> energy \<equiv> {\<phi> . expressiveness_price \<phi> \<le> energy}"
 
-fun expr_pr_\<chi> :: "('a, 's) hml_srbb_inner \<Rightarrow> energy" where
-  "expr_pr_\<chi> \<chi> = E (modal_depth_srbb_inner \<chi>)
-                 (branch_conj_depth_\<chi> \<chi>)
-                 (inst_conj_depth_\<chi> \<chi>)
-                 (st_conj_depth_\<chi> \<chi>)
-                 (imm_conj_depth_\<chi> \<chi>)
-                 (max_pos_conj_depth_\<chi> \<chi>)
-                 (max_neg_conj_depth_\<chi> \<chi>)
-                 (neg_depth_\<chi> \<chi>)"
+fun expr_pr_inner :: "('a, 's) hml_srbb_inner \<Rightarrow> energy" where
+  "expr_pr_inner \<chi> = E (modal_depth_srbb_inner \<chi>)
+                 (branch_conj_depth_inner \<chi>)
+                 (inst_conj_depth_inner \<chi>)
+                 (st_conj_depth_inner \<chi>)
+                 (imm_conj_depth_inner \<chi>)
+                 (max_pos_conj_depth_inner \<chi>)
+                 (max_neg_conj_depth_inner \<chi>)
+                 (neg_depth_inner \<chi>)"
 
-lemma \<chi>_price_never_neg: "expr_pr_\<chi> \<chi> \<noteq> eneg"
+lemma \<chi>_price_never_neg: "expr_pr_inner \<chi> \<noteq> eneg"
   by simp
 
-definition \<O>_\<chi> :: "energy \<Rightarrow> (('a, 's) hml_srbb_inner) set" where
-  "\<O>_\<chi> energy \<equiv> {\<chi> . expr_pr_\<chi> \<chi> \<le> energy}"
+definition \<O>_inner :: "energy \<Rightarrow> (('a, 's) hml_srbb_inner) set" where
+  "\<O>_inner energy \<equiv> {\<chi> . expr_pr_inner \<chi> \<le> energy}"
 
 subsection \<open>characterizing equivalence by energy coordinates\<close>
 
